
%----------------------------------------------------------------------------------------
%	Lecture 4
%----------------------------------------------------------------------------------------

\section*{\centering Chain Rule}  

\bigbreak
\section{Chain Rule}

We've got a general procedure for differentiating expressions with addition, subtraction, multiplication and division.
What about \underline{composition}?

\subsubsection*{Differentiating composition : $y = f(x) = \sin x , x = g(t) = t^2.$}

So, $y = f(g(t)) = \sin t^2$. To find $\diff{y}{t}$, write
$$ \frac{\Delta y}{\Delta t} = \frac{\Delta y}{\Delta x} \cdot \frac{\Delta x}{\Delta t} $$

As $\Delta t \to 0, \Delta x \to 0$ too, because of continuity. So we get : 
$$ \diff{y}{t} = \diff{y}{x} \diff{x}{t} \leftarrow \textbf{The Chain Rule!} $$

In this example, $\diff{x}{t} = 2t$ and $\diff{y}{x} = \cos x$.
\begin{equation*}
\begin{split}
	\text{So, $\quad$} \diff{}{t} \sin(t^2) 
		& = (\diff{y}{x})(\diff{x}{t}) \\
		& = (\cos x)(2t) \\
		& = (2t)(\cos(x^2)) \\
\end{split}
\end{equation*}

\subsubsection*{Another Notation for Chain Rule}

$$ \diff{}{t}f(g(t)) = f'(g(t))g'(t) $$
$$ \text{Note : } f \circ g \neq g \circ f $$

\subsubsection*{Extending Power Rule : $\diff{}{x} x^n = nx^{n-1}$ for $n = 0, -1, -2, -3\ldots$}

There are two ways to proceed. $x^{-n} = \left( \frac{1}{x} \right)^n$, or $x^{-n} = \frac{1}{x^n}$

\begin{enumerate}
	\item $ \diff{}{x} (x^{-n}) 
		= \diff{}{x} \left( \frac{1}{x} \right)^n 
		= n \left( \frac{1}{x} \right)^{n-1} \left( \frac{-1}{x^2} \right) 
		= -nx^{-(n-1)}x^{-2}
		= -nx^{-n-1}
		$
	\item $ \diff{}{x} (x^{-n}) 
		= \diff{}{x} \left( \frac{1}{x^n} \right)
		= nx^{n-1} \left( \frac{-1}{x^{2n}} \right)
		= -nx^{-n-1}
		$
	\item $ \diff{}{x} x^0 = \diff{}{x} 1 = 0 = 0x^{0-1} $
\end{enumerate}



Thus, $$ \diff{}{x} x^n = nx^{n-1} \text{ for } n = \ldots -2, -1, 0, 1, 2, \ldots $$